ch32-string-matching/test_without_lemma.fst
@@ -1,0 +1,8 @@
+module TestWithoutLemma
+open CLRS.Ch32.RabinKarp.Spec
+
+// Test that we can use the functions
+let test () = 
+  let text = Seq.seq_of_list [1;2;3;4] in
+  let pattern = Seq.seq_of_list [2;3] in
+  rabin_karp_find_all text pattern 10 13
